NuStd_Base.thy
@@ -82,21 +82,21 @@ declare [ [\<phi>not_define_new_const] ]
 proc op_get_var:
   assumes [unfolded \<phi>SemType_def subset_iff, useful]: \<open>\<phi>SemType (x \<Ztypecolon> T) TY\<close>
   argument \<open>x \<Ztypecolon> Var vname T\<close>
-  return   \<open>x \<Ztypecolon> Var vname T\<heavy_comma> x \<Ztypecolon> \<^bold>v\<^bold>a\<^bold>l T\<close>
+  return   \<open>x \<Ztypecolon> Var vname T\<heavy_comma> \<^bold>v\<^bold>a\<^bold>l x \<Ztypecolon> T\<close>
   \<medium_left_bracket>
     to_Identity op_get_var''
   \<medium_right_bracket>. .
 
-declare [ [\<phi>trace_reasoning] ]
 
 lemma [\<phi>reason on \<open>\<^bold>p\<^bold>r\<^bold>o\<^bold>c ?f \<lbrace> ?R \<longmapsto> \<lambda>ret. ?R'\<heavy_comma> SYNTHESIS ?x <val-of-var> ?var \<Ztypecolon> ?T ret \<^bold>t\<^bold>h\<^bold>r\<^bold>o\<^bold>w\<^bold>s ?E \<rbrace> \<^bold>@\<^bold>G\<^bold>O\<^bold>A\<^bold>L ?G\<close>]:
   \<open> SUBGOAL G G2
 \<Longrightarrow> \<^bold>s\<^bold>u\<^bold>b\<^bold>t\<^bold>y\<^bold>p\<^bold>e X \<longmapsto> Y\<heavy_comma> \<blangle> x \<Ztypecolon> Var var T \<brangle> \<^bold>@\<^bold>G\<^bold>O\<^bold>A\<^bold>L G2
 \<Longrightarrow> SOLVE_SUBGOAL G2
 \<Longrightarrow> \<phi>SemType (x \<Ztypecolon> T) TY
-\<Longrightarrow> \<^bold>p\<^bold>r\<^bold>o\<^bold>c op_get_var var TY \<lbrace> X \<longmapsto> Y\<heavy_comma> x \<Ztypecolon> Var var T \<heavy_comma> SYNTHESIS x <val-of-var> var \<Ztypecolon> \<^bold>v\<^bold>a\<^bold>l T \<rbrace> \<^bold>@\<^bold>G\<^bold>O\<^bold>A\<^bold>L G\<close>
+\<Longrightarrow> \<^bold>p\<^bold>r\<^bold>o\<^bold>c op_get_var var TY \<lbrace> X \<longmapsto> Y\<heavy_comma> x \<Ztypecolon> Var var T \<heavy_comma> SYNTHESIS \<^bold>v\<^bold>a\<^bold>l x <val-of-var> var \<Ztypecolon> T \<rbrace> \<^bold>@\<^bold>G\<^bold>O\<^bold>A\<^bold>L G\<close>
   \<medium_left_bracket> premises _ and GetVar and _ and [\<phi>reason on \<open>\<phi>SemType (x \<Ztypecolon> T) ?TY\<close>]
     GetVar op_get_var \<medium_right_bracket>. .
+
 
 
 paragraph \<open>Set Variable\<close>
@@ -104,14 +104,14 @@ paragraph \<open>Set Variable\<close>
 proc op_set_var:
   assumes [unfolded \<phi>SemType_def subset_iff, useful]: \<open>\<phi>SemType (x \<Ztypecolon> T) TY\<close>
   assumes [unfolded \<phi>SemType_def subset_iff, useful]: \<open>\<phi>SemType (y \<Ztypecolon> U) TY\<close>
-  argument \<open>x \<Ztypecolon> Var var T\<heavy_comma> y \<Ztypecolon> \<^bold>v\<^bold>a\<^bold>l U\<close>
+  argument \<open>x \<Ztypecolon> Var var T\<heavy_comma> \<^bold>v\<^bold>a\<^bold>l y \<Ztypecolon> U\<close>
   return   \<open>y \<Ztypecolon> Var var U\<close>
   \<medium_left_bracket> to_Identity \<open>var\<close> to_Identity op_set_var'' \<medium_right_bracket>. .
 
 proc op_set_var__synthesis[
   \<phi>reason on \<open>\<^bold>p\<^bold>r\<^bold>o\<^bold>c ?f \<lbrace> ?R \<longmapsto> \<lambda>ret. ?R'\<heavy_comma> SYNTHESIS ($?var := ?y) \<Ztypecolon> ?U ret \<^bold>t\<^bold>h\<^bold>r\<^bold>o\<^bold>w\<^bold>s ?E \<rbrace> \<^bold>@\<^bold>G\<^bold>O\<^bold>A\<^bold>L ?G\<close>
 ]:
-assumes G: \<open>\<^bold>p\<^bold>r\<^bold>o\<^bold>c g \<lbrace> X \<longmapsto> X1\<heavy_comma> SYNTHESIS y \<Ztypecolon> \<^bold>v\<^bold>a\<^bold>l U \<^bold>t\<^bold>h\<^bold>r\<^bold>o\<^bold>w\<^bold>s E\<rbrace> \<^bold>@\<^bold>G\<^bold>O\<^bold>A\<^bold>L G \<close>
+assumes G: \<open>\<^bold>p\<^bold>r\<^bold>o\<^bold>c g \<lbrace> X \<longmapsto> X1\<heavy_comma> SYNTHESIS \<^bold>v\<^bold>a\<^bold>l y \<Ztypecolon> U \<^bold>t\<^bold>h\<^bold>r\<^bold>o\<^bold>w\<^bold>s E\<rbrace> \<^bold>@\<^bold>G\<^bold>O\<^bold>A\<^bold>L G \<close>
   and      \<open>SUBGOAL G G2\<close>
   and S[unfolded GOAL_CTXT_def FOCUS_TAG_def]:
         \<open>\<And>vy. \<^bold>s\<^bold>u\<^bold>b\<^bold>t\<^bold>y\<^bold>p\<^bold>e X1\<heavy_comma> y \<Ztypecolon> Val vy U \<longmapsto> \<blangle> Y\<heavy_comma> x \<Ztypecolon> Var var T\<heavy_comma> y \<Ztypecolon> Val vy U \<brangle> \<^bold>w\<^bold>i\<^bold>t\<^bold>h Any \<^bold>@\<^bold>G\<^bold>O\<^bold>A\<^bold>L G2\<close>
@@ -120,7 +120,7 @@ assumes G: \<open>\<^bold>p\<^bold>r\<^bold>o\<^bold>c g \<lbrace> X \<longmapst
   and [\<phi>reason on \<open>\<phi>SemType (y \<Ztypecolon> U) ?TY\<close>]: \<open>\<phi>SemType (y \<Ztypecolon> U) TY\<close>
  goal G
 argument \<open>X\<close>
-return   \<open>Y\<heavy_comma> y \<Ztypecolon> Var var U \<heavy_comma> SYNTHESIS ($var := y) \<Ztypecolon> \<^bold>v\<^bold>a\<^bold>l U\<close>
+return   \<open>Y\<heavy_comma> y \<Ztypecolon> Var var U \<heavy_comma> SYNTHESIS \<^bold>v\<^bold>a\<^bold>l ($var := y) \<Ztypecolon> U\<close>
 throws   E
   \<medium_left_bracket> G S op_set_var op_get_var \<medium_right_bracket>. .
 
@@ -128,30 +128,32 @@ declare [ [\<phi>not_define_new_const = false] ]
 
 paragraph \<open>Declare New Variables\<close>
 
+declare [ [\<phi>trace_reasoning] ]
+
 proc (in std) op_var_scope:
   assumes [unfolded \<phi>SemType_def subset_iff, useful]: \<open>\<phi>SemType (x \<Ztypecolon> T) TY\<close>
     and BLK: \<open>\<forall>var. \<^bold>p\<^bold>r\<^bold>o\<^bold>c F var \<lbrace> X\<heavy_comma> x \<Ztypecolon> Var var T \<longmapsto> \<lambda>ret. Y ret\<heavy_comma> y \<Ztypecolon> Var var (U <of-type> TY) \<^bold>t\<^bold>h\<^bold>r\<^bold>o\<^bold>w\<^bold>s E\<heavy_comma> y \<Ztypecolon> Var var (U <of-type> TY) \<rbrace>\<close>
-  argument \<open>X\<heavy_comma> x \<Ztypecolon> \<^bold>v\<^bold>a\<^bold>l T\<close>
+  argument \<open>X\<heavy_comma> \<^bold>v\<^bold>a\<^bold>l x \<Ztypecolon> T\<close>
   return   \<open>Y\<close>
   throws   E
   \<medium_left_bracket> to_Identity op_var_scope';;
-    try'' \<medium_left_bracket> BLK to_Identity op_free_var \<medium_right_bracket>. \<medium_left_bracket> to_Identity op_free_var;; throw \<medium_right_bracket>. \<medium_right_bracket>. .
+    try'' ;; \<medium_left_bracket> BLK to_Identity op_free_var \<medium_right_bracket> .. \<medium_left_bracket> to_Identity op_free_var;; throw \<medium_right_bracket>. \<medium_right_bracket>. .
 
 
 lemma "__\<phi>op_var_scope__":
-  \<open> (\<And>var. \<^bold>p\<^bold>r\<^bold>o\<^bold>c F var \<lbrace> R\<heavy_comma> x \<Ztypecolon> Var var T\<heavy_comma>  X \<longmapsto> Y \<^bold>r\<^bold>e\<^bold>t \<heavy_comma> y \<Ztypecolon> Var var (U <of-type> TY) \<^bold>t\<^bold>h\<^bold>r\<^bold>o\<^bold>w\<^bold>s E\<heavy_comma> y \<Ztypecolon> Var var (U <of-type> TY) \<rbrace>)
+  \<open> (\<And>var. \<^bold>p\<^bold>r\<^bold>o\<^bold>c F var \<lbrace> R\<heavy_comma> x \<Ztypecolon> Var var T\<heavy_comma>  X \<longmapsto> Y (ret::'aa sem_value) \<heavy_comma> y \<Ztypecolon> Var var (U <of-type> TY) \<^bold>t\<^bold>h\<^bold>r\<^bold>o\<^bold>w\<^bold>s E\<heavy_comma> y \<Ztypecolon> Var var (U <of-type> TY) \<rbrace>)
 \<Longrightarrow> \<phi>SemType (x \<Ztypecolon> T) TY
-\<Longrightarrow> \<^bold>p\<^bold>r\<^bold>o\<^bold>c op_var_scope TY F [raw] \<lbrace> R\<heavy_comma> (X\<heavy_comma> x \<Ztypecolon> Val raw T) \<longmapsto> Y \<^bold>r\<^bold>e\<^bold>t \<^bold>t\<^bold>h\<^bold>r\<^bold>o\<^bold>w\<^bold>s E \<rbrace>\<close>
+\<Longrightarrow> \<^bold>p\<^bold>r\<^bold>o\<^bold>c op_var_scope TYPE('a) TY F raw \<lbrace> R\<heavy_comma> (X\<heavy_comma> x \<Ztypecolon> Val raw T) \<longmapsto> Y (ret::'aa sem_value) \<^bold>t\<^bold>h\<^bold>r\<^bold>o\<^bold>w\<^bold>s E \<rbrace>\<close>
   unfolding mult.assoc[symmetric]
   using op_var_scope_\<phi>app[where X=\<open>R\<heavy_comma> X\<close> and x = x and T = T and TY = TY and F=F and y=y,
-            of Y U E \<open>[raw]\<close>, simplified]
+            of Y U E \<open>raw\<close>, simplified]
   by (smt (verit, best) ab_semigroup_mult_class.mult_ac(1) mult.commute)
 
 lemma "__\<phi>op_set_var__":
   \<open> \<^bold>p\<^bold>r\<^bold>o\<^bold>c g \<lbrace> R\<heavy_comma> y \<Ztypecolon> Var var U\<heavy_comma> X \<longmapsto> Z \<^bold>t\<^bold>h\<^bold>r\<^bold>o\<^bold>w\<^bold>s E \<rbrace>
 \<Longrightarrow> \<phi>SemType (x \<Ztypecolon> T) TY
 \<Longrightarrow> \<phi>SemType (y \<Ztypecolon> U) TY
-\<Longrightarrow> \<^bold>p\<^bold>r\<^bold>o\<^bold>c (op_set_var var TY [raw] \<ggreater> g) \<lbrace> R\<heavy_comma> (X\<heavy_comma> x \<Ztypecolon> Var var T \<heavy_comma> y \<Ztypecolon> Val raw U) \<longmapsto> Z \<^bold>t\<^bold>h\<^bold>r\<^bold>o\<^bold>w\<^bold>s E \<rbrace>\<close>
+\<Longrightarrow> \<^bold>p\<^bold>r\<^bold>o\<^bold>c (op_set_var var TY raw \<ggreater> g) \<lbrace> R\<heavy_comma> (X\<heavy_comma> x \<Ztypecolon> Var var T \<heavy_comma> y \<Ztypecolon> Val raw U) \<longmapsto> Z \<^bold>t\<^bold>h\<^bold>r\<^bold>o\<^bold>w\<^bold>s E \<rbrace>\<close>
   \<medium_left_bracket> premises G and [\<phi>reason on \<open>\<phi>SemType (x \<Ztypecolon> T) ?TY\<close>] and [\<phi>reason on \<open>\<phi>SemType (y \<Ztypecolon> U) ?TY\<close>]
     op_set_var G \<medium_right_bracket>. .
 
@@ -181,62 +183,61 @@ subsubsection \<open>Boolean Arithmetic\<close>
 paragraph \<open>Not\<close>
 
 lemma (in std) op_not[\<phi>overload \<not>]:
-  \<open>\<^bold>p\<^bold>r\<^bold>o\<^bold>c op_not [raw] \<lbrace> x \<Ztypecolon> Val raw \<bool> \<longmapsto> \<not> x \<Ztypecolon> \<^bold>v\<^bold>a\<^bold>l \<bool> \<rbrace>\<close>
+  \<open>\<^bold>p\<^bold>r\<^bold>o\<^bold>c op_not raw \<lbrace> x \<Ztypecolon> Val raw \<bool> \<longmapsto> \<^bold>v\<^bold>a\<^bold>l \<not> x \<Ztypecolon> \<bool> \<rbrace>\<close>
   unfolding op_not_def
-  by \<phi>reason
+  by (cases raw, simp, \<phi>reason)
 
 proc "\<phi>__synthesis_lneg"[
     \<phi>reason on \<open>\<^bold>p\<^bold>r\<^bold>o\<^bold>c ?F \<lbrace> ?R \<longmapsto> \<lambda>ret. ?R1\<heavy_comma> SYNTHESIS \<not>?b \<Ztypecolon> ?T ret \<^bold>t\<^bold>h\<^bold>r\<^bold>o\<^bold>w\<^bold>s ?E \<rbrace> \<^bold>@\<^bold>G\<^bold>O\<^bold>A\<^bold>L ?G\<close>
 ]:
-  assumes F1: \<open>\<^bold>p\<^bold>r\<^bold>o\<^bold>c f \<lbrace> R \<longmapsto> R1\<heavy_comma> SYNTHESIS b \<Ztypecolon> \<^bold>v\<^bold>a\<^bold>l \<bool> \<rbrace>  \<^bold>@\<^bold>G\<^bold>O\<^bold>A\<^bold>L G\<close>
+  assumes F1: \<open>\<^bold>p\<^bold>r\<^bold>o\<^bold>c f \<lbrace> R \<longmapsto> R1\<heavy_comma> SYNTHESIS \<^bold>v\<^bold>a\<^bold>l b \<Ztypecolon> \<bool> \<rbrace>  \<^bold>@\<^bold>G\<^bold>O\<^bold>A\<^bold>L G\<close>
   goal G
   argument \<open>R\<close>
-  return   \<open>R1\<heavy_comma> SYNTHESIS \<not>b \<Ztypecolon> \<^bold>v\<^bold>a\<^bold>l \<bool>\<close>
+  return   \<open>R1\<heavy_comma> SYNTHESIS \<^bold>v\<^bold>a\<^bold>l \<not>b \<Ztypecolon> \<bool>\<close>
   \<medium_left_bracket> F1 \<not> \<medium_right_bracket>. .
 
 paragraph \<open>And\<close>
 
 lemma (in std) op_and[\<phi>overload \<and>]:
-  \<open>\<^bold>p\<^bold>r\<^bold>o\<^bold>c op_and [vb,va] \<lbrace> a \<Ztypecolon> Val va \<bool>\<heavy_comma> b \<Ztypecolon> Val vb \<bool> \<longmapsto> a \<and> b \<Ztypecolon> \<^bold>v\<^bold>a\<^bold>l \<bool> \<rbrace>\<close>
+  \<open>\<^bold>p\<^bold>r\<^bold>o\<^bold>c op_and (\<phi>V_pair vb va) \<lbrace> a \<Ztypecolon> Val va \<bool>\<heavy_comma> b \<Ztypecolon> Val vb \<bool> \<longmapsto> \<^bold>v\<^bold>a\<^bold>l a \<and> b \<Ztypecolon> \<bool> \<rbrace>\<close>
   unfolding op_and_def
-  by \<phi>reason
+  by (cases va; cases vb; simp, \<phi>reason)
 
 proc "\<phi>__synthesis_land"[
     \<phi>reason on \<open>\<^bold>p\<^bold>r\<^bold>o\<^bold>c ?F \<lbrace> ?R \<longmapsto> \<lambda>ret. ?R2\<heavy_comma> SYNTHESIS (?x \<and> ?y) \<Ztypecolon> ?T ret \<^bold>t\<^bold>h\<^bold>r\<^bold>o\<^bold>w\<^bold>s ?E \<rbrace> \<^bold>@\<^bold>G\<^bold>O\<^bold>A\<^bold>L ?G\<close>
 ]:
-  assumes F1: \<open>\<^bold>p\<^bold>r\<^bold>o\<^bold>c f1 \<lbrace> R \<longmapsto> R1\<heavy_comma> SYNTHESIS y \<Ztypecolon> \<^bold>v\<^bold>a\<^bold>l \<bool> \<^bold>t\<^bold>h\<^bold>r\<^bold>o\<^bold>w\<^bold>s E1 \<rbrace>  \<^bold>@\<^bold>G\<^bold>O\<^bold>A\<^bold>L G\<close>
-    and   F2: \<open>\<^bold>p\<^bold>r\<^bold>o\<^bold>c f2 \<lbrace> R1 \<longmapsto> R2\<heavy_comma> SYNTHESIS x \<Ztypecolon> \<^bold>v\<^bold>a\<^bold>l \<bool> \<^bold>t\<^bold>h\<^bold>r\<^bold>o\<^bold>w\<^bold>s E2 \<rbrace>  \<^bold>@\<^bold>G\<^bold>O\<^bold>A\<^bold>L G\<close>
+  assumes F1: \<open>\<^bold>p\<^bold>r\<^bold>o\<^bold>c f1 \<lbrace> R  \<longmapsto> R1\<heavy_comma> SYNTHESIS \<^bold>v\<^bold>a\<^bold>l y \<Ztypecolon> \<bool> \<^bold>t\<^bold>h\<^bold>r\<^bold>o\<^bold>w\<^bold>s E1 \<rbrace>  \<^bold>@\<^bold>G\<^bold>O\<^bold>A\<^bold>L G\<close>
+    and   F2: \<open>\<^bold>p\<^bold>r\<^bold>o\<^bold>c f2 \<lbrace> R1 \<longmapsto> R2\<heavy_comma> SYNTHESIS \<^bold>v\<^bold>a\<^bold>l x \<Ztypecolon> \<bool> \<^bold>t\<^bold>h\<^bold>r\<^bold>o\<^bold>w\<^bold>s E2 \<rbrace>  \<^bold>@\<^bold>G\<^bold>O\<^bold>A\<^bold>L G\<close>
   goal G
   argument \<open>R\<close>
-  return   \<open>R2\<heavy_comma> SYNTHESIS (x \<and> y) \<Ztypecolon> \<^bold>v\<^bold>a\<^bold>l \<bool>\<close>
+  return   \<open>R2\<heavy_comma> SYNTHESIS \<^bold>v\<^bold>a\<^bold>l (x \<and> y) \<Ztypecolon> \<bool>\<close>
   throws   \<open>E1 + E2\<close>
-  \<medium_left_bracket> F1 \<rightarrow> y ;; F2 ;; $y ;; \<and> ;; \<medium_right_bracket>. .
+  \<medium_left_bracket> F1 \<rightarrow> y;; F2 $y \<and>  \<medium_right_bracket>. .
 
 paragraph \<open>Or\<close>
 
 lemma (in std) op_or[\<phi>overload \<or>]:
-  \<open>\<^bold>p\<^bold>r\<^bold>o\<^bold>c op_or [vb,va] \<lbrace> a \<Ztypecolon> Val va \<bool>\<heavy_comma> b \<Ztypecolon> Val vb \<bool> \<longmapsto> a \<or> b \<Ztypecolon> \<^bold>v\<^bold>a\<^bold>l \<bool> \<rbrace>\<close>
+  \<open>\<^bold>p\<^bold>r\<^bold>o\<^bold>c op_or (\<phi>V_pair vb va) \<lbrace> a \<Ztypecolon> Val va \<bool>\<heavy_comma> b \<Ztypecolon> Val vb \<bool> \<longmapsto> \<^bold>v\<^bold>a\<^bold>l a \<or> b \<Ztypecolon> \<bool> \<rbrace>\<close>
   unfolding op_or_def
-  by \<phi>reason
+  by (cases va; cases vb, simp, \<phi>reason)
 
-declare [ [\<phi>trace_reasoning] ]
 
 proc \<phi>__synthesis_lor[
-    \<phi>reason on \<open>\<^bold>p\<^bold>r\<^bold>o\<^bold>c ?F \<lbrace> ?R \<longmapsto> ?R2\<heavy_comma> SYNTHESIS VAL (?x \<or> ?y) \<Ztypecolon> ?T \<^bold>t\<^bold>h\<^bold>r\<^bold>o\<^bold>w\<^bold>s ?E \<rbrace> \<^bold>@\<^bold>G\<^bold>O\<^bold>A\<^bold>L ?G\<close>
+    \<phi>reason on \<open>\<^bold>p\<^bold>r\<^bold>o\<^bold>c ?F \<lbrace> ?R \<longmapsto> \<lambda>ret. ?R2\<heavy_comma> SYNTHESIS (?x \<or> ?y) \<Ztypecolon> ?T ret \<^bold>t\<^bold>h\<^bold>r\<^bold>o\<^bold>w\<^bold>s ?E \<rbrace> \<^bold>@\<^bold>G\<^bold>O\<^bold>A\<^bold>L ?G\<close>
 ]:
-  assumes F1: \<open>\<^bold>p\<^bold>r\<^bold>o\<^bold>c f1 \<lbrace> R \<longmapsto> R1\<heavy_comma> y \<Ztypecolon> \<^bold>v\<^bold>a\<^bold>l \<bool>\<heavy_comma> SYNTHESIS y \<Ztypecolon> \<^bold>v\<^bold>a\<^bold>l \<bool> \<^bold>t\<^bold>h\<^bold>r\<^bold>o\<^bold>w\<^bold>s E1 \<rbrace>  \<^bold>@\<^bold>G\<^bold>O\<^bold>A\<^bold>L G\<close>
-    and   F2: \<open>\<^bold>p\<^bold>r\<^bold>o\<^bold>c f2 \<lbrace> R1 \<longmapsto> R2\<heavy_comma> SYNTHESIS x \<Ztypecolon> \<^bold>v\<^bold>a\<^bold>l \<bool> \<^bold>t\<^bold>h\<^bold>r\<^bold>o\<^bold>w\<^bold>s E2 \<rbrace>  \<^bold>@\<^bold>G\<^bold>O\<^bold>A\<^bold>L G\<close>
+  assumes F1: \<open>\<^bold>p\<^bold>r\<^bold>o\<^bold>c f1 \<lbrace> R \<longmapsto> R1\<heavy_comma> SYNTHESIS \<^bold>v\<^bold>a\<^bold>l y \<Ztypecolon> \<bool> \<^bold>t\<^bold>h\<^bold>r\<^bold>o\<^bold>w\<^bold>s E1 \<rbrace>  \<^bold>@\<^bold>G\<^bold>O\<^bold>A\<^bold>L G\<close>
+    and   F2: \<open>\<^bold>p\<^bold>r\<^bold>o\<^bold>c f2 \<lbrace> R1 \<longmapsto> R2\<heavy_comma> SYNTHESIS \<^bold>v\<^bold>a\<^bold>l x \<Ztypecolon> \<bool> \<^bold>t\<^bold>h\<^bold>r\<^bold>o\<^bold>w\<^bold>s E2 \<rbrace>  \<^bold>@\<^bold>G\<^bold>O\<^bold>A\<^bold>L G\<close>
   goal G
   argument \<open>R\<close>
-  return   \<open>R2\<heavy_comma> SYNTHESIS (x \<or> y) \<Ztypecolon> \<^bold>v\<^bold>a\<^bold>l \<bool>\<close>
+  return   \<open>R2\<heavy_comma> SYNTHESIS \<^bold>v\<^bold>a\<^bold>l (x \<or> y) \<Ztypecolon> \<bool>\<close>
   throws \<open>E1 + E2\<close>
-  \<medium_left_bracket> F1 ;; \<rightarrow> y;; F2 ;; $y \<or> \<medium_right_bracket> .. .
+  \<medium_left_bracket> F1 \<rightarrow> y;; F2 $y \<or> \<medium_right_bracket>. .
 
 
 subsubsection \<open>Constant Integer\<close>
 
 lemma (in std) op_const_int_\<phi>app:
-  \<open>\<^bold>p\<^bold>r\<^bold>e\<^bold>m\<^bold>i\<^bold>s\<^bold>e n < 2^b \<Longrightarrow> \<^bold>p\<^bold>r\<^bold>o\<^bold>c op_const_int b n \<lbrace> Void \<longmapsto> n \<Ztypecolon> \<^bold>v\<^bold>a\<^bold>l \<nat>[b] \<rbrace>\<close>
+  \<open>\<^bold>p\<^bold>r\<^bold>e\<^bold>m\<^bold>i\<^bold>s\<^bold>e n < 2^b \<Longrightarrow> \<^bold>p\<^bold>r\<^bold>o\<^bold>c op_const_int b n \<lbrace> Void \<longmapsto> \<^bold>v\<^bold>a\<^bold>l n \<Ztypecolon> \<nat>[b] \<rbrace>\<close>
   unfolding op_const_int_def Premise_def Synthesis_def
   by \<phi>reason
 
@@ -249,26 +250,26 @@ lemma (in std) [\<phi>reason 1200
   unfolding Synthesis_Parse_def ..
 
 lemma (in std) [\<phi>reason
-    on \<open>\<^bold>p\<^bold>r\<^bold>o\<^bold>c ?f \<lbrace> ?X' \<longmapsto> ?X\<heavy_comma> SYNTHESIS numeral ?n \<Ztypecolon> \<nat>[?b] \<^bold>t\<^bold>h\<^bold>r\<^bold>o\<^bold>w\<^bold>s ?E \<rbrace> \<^bold>@\<^bold>G\<^bold>O\<^bold>A\<^bold>L ?G\<close>
-       \<open>\<^bold>p\<^bold>r\<^bold>o\<^bold>c ?f \<lbrace> ?X' \<longmapsto> ?X\<heavy_comma> SYNTHESIS 1 \<Ztypecolon> \<nat>[?b] \<^bold>t\<^bold>h\<^bold>r\<^bold>o\<^bold>w\<^bold>s ?E \<rbrace> \<^bold>@\<^bold>G\<^bold>O\<^bold>A\<^bold>L ?G\<close>
-       \<open>\<^bold>p\<^bold>r\<^bold>o\<^bold>c ?f \<lbrace> ?X' \<longmapsto> ?X\<heavy_comma> SYNTHESIS 0 \<Ztypecolon> \<nat>[?b] \<^bold>t\<^bold>h\<^bold>r\<^bold>o\<^bold>w\<^bold>s ?E \<rbrace> \<^bold>@\<^bold>G\<^bold>O\<^bold>A\<^bold>L ?G\<close>
+    on \<open>\<^bold>p\<^bold>r\<^bold>o\<^bold>c ?f \<lbrace> ?X' \<longmapsto> ?X\<heavy_comma> SYNTHESIS \<^bold>v\<^bold>a\<^bold>l numeral ?n \<Ztypecolon> \<nat>[?b] \<^bold>t\<^bold>h\<^bold>r\<^bold>o\<^bold>w\<^bold>s ?E \<rbrace> \<^bold>@\<^bold>G\<^bold>O\<^bold>A\<^bold>L ?G\<close>
+       \<open>\<^bold>p\<^bold>r\<^bold>o\<^bold>c ?f \<lbrace> ?X' \<longmapsto> ?X\<heavy_comma> SYNTHESIS \<^bold>v\<^bold>a\<^bold>l 1 \<Ztypecolon> \<nat>[?b] \<^bold>t\<^bold>h\<^bold>r\<^bold>o\<^bold>w\<^bold>s ?E \<rbrace> \<^bold>@\<^bold>G\<^bold>O\<^bold>A\<^bold>L ?G\<close>
+       \<open>\<^bold>p\<^bold>r\<^bold>o\<^bold>c ?f \<lbrace> ?X' \<longmapsto> ?X\<heavy_comma> SYNTHESIS \<^bold>v\<^bold>a\<^bold>l 0 \<Ztypecolon> \<nat>[?b] \<^bold>t\<^bold>h\<^bold>r\<^bold>o\<^bold>w\<^bold>s ?E \<rbrace> \<^bold>@\<^bold>G\<^bold>O\<^bold>A\<^bold>L ?G\<close>
 ]:
   \<open> \<^bold>p\<^bold>r\<^bold>e\<^bold>m\<^bold>i\<^bold>s\<^bold>e n < 2^b
-\<Longrightarrow> \<^bold>p\<^bold>r\<^bold>o\<^bold>c op_const_int b n \<lbrace> R \<longmapsto> R\<heavy_comma> SYNTHESIS n \<Ztypecolon> \<nat>[b] \<rbrace> \<^bold>@\<^bold>G\<^bold>O\<^bold>A\<^bold>L G\<close>
+\<Longrightarrow> \<^bold>p\<^bold>r\<^bold>o\<^bold>c op_const_int b n \<lbrace> R \<longmapsto> R\<heavy_comma> SYNTHESIS \<^bold>v\<^bold>a\<^bold>l n \<Ztypecolon> \<nat>[b] \<rbrace> \<^bold>@\<^bold>G\<^bold>O\<^bold>A\<^bold>L G\<close>
   unfolding Synthesis_def GOAL_CTXT_def
   using op_const_int_\<phi>app[THEN \<phi>frame, simplified] .
 
 lemma (in std) op_const_size_t:
-  \<open>\<^bold>p\<^bold>r\<^bold>o\<^bold>c op_const_size_t n \<lbrace> Void \<longmapsto> n \<Ztypecolon> \<^bold>v\<^bold>a\<^bold>l Size \<rbrace>\<close>
+  \<open>\<^bold>p\<^bold>r\<^bold>o\<^bold>c op_const_size_t n \<lbrace> Void \<longmapsto> \<^bold>v\<^bold>a\<^bold>l n \<Ztypecolon> Size \<rbrace>\<close>
   unfolding op_const_size_t_def Premise_def
   by \<phi>reason
 
 lemma (in std) [\<phi>reason 1200
-    on \<open>\<^bold>p\<^bold>r\<^bold>o\<^bold>c ?f \<lbrace> ?X' \<longmapsto> ?X\<heavy_comma> SYNTHESIS (numeral ?n) \<Ztypecolon> Size \<^bold>t\<^bold>h\<^bold>r\<^bold>o\<^bold>w\<^bold>s ?E \<rbrace> \<^bold>@\<^bold>G\<^bold>O\<^bold>A\<^bold>L ?G\<close>
-       \<open>\<^bold>p\<^bold>r\<^bold>o\<^bold>c ?f \<lbrace> ?X' \<longmapsto> ?X\<heavy_comma> SYNTHESIS 0 \<Ztypecolon> Size \<^bold>t\<^bold>h\<^bold>r\<^bold>o\<^bold>w\<^bold>s ?E \<rbrace> \<^bold>@\<^bold>G\<^bold>O\<^bold>A\<^bold>L ?G\<close>
-       \<open>\<^bold>p\<^bold>r\<^bold>o\<^bold>c ?f \<lbrace> ?X' \<longmapsto> ?X\<heavy_comma> SYNTHESIS 1 \<Ztypecolon> Size \<^bold>t\<^bold>h\<^bold>r\<^bold>o\<^bold>w\<^bold>s ?E \<rbrace> \<^bold>@\<^bold>G\<^bold>O\<^bold>A\<^bold>L ?G\<close>
+    on \<open>\<^bold>p\<^bold>r\<^bold>o\<^bold>c ?f \<lbrace> ?X' \<longmapsto> ?X\<heavy_comma> SYNTHESIS \<^bold>v\<^bold>a\<^bold>l (numeral ?n) \<Ztypecolon> Size \<^bold>t\<^bold>h\<^bold>r\<^bold>o\<^bold>w\<^bold>s ?E \<rbrace> \<^bold>@\<^bold>G\<^bold>O\<^bold>A\<^bold>L ?G\<close>
+       \<open>\<^bold>p\<^bold>r\<^bold>o\<^bold>c ?f \<lbrace> ?X' \<longmapsto> ?X\<heavy_comma> SYNTHESIS \<^bold>v\<^bold>a\<^bold>l 0 \<Ztypecolon> Size \<^bold>t\<^bold>h\<^bold>r\<^bold>o\<^bold>w\<^bold>s ?E \<rbrace> \<^bold>@\<^bold>G\<^bold>O\<^bold>A\<^bold>L ?G\<close>
+       \<open>\<^bold>p\<^bold>r\<^bold>o\<^bold>c ?f \<lbrace> ?X' \<longmapsto> ?X\<heavy_comma> SYNTHESIS \<^bold>v\<^bold>a\<^bold>l 1 \<Ztypecolon> Size \<^bold>t\<^bold>h\<^bold>r\<^bold>o\<^bold>w\<^bold>s ?E \<rbrace> \<^bold>@\<^bold>G\<^bold>O\<^bold>A\<^bold>L ?G\<close>
 ]:
-  \<open>\<^bold>p\<^bold>r\<^bold>o\<^bold>c op_const_size_t n \<lbrace> R \<longmapsto> R\<heavy_comma> SYNTHESIS n \<Ztypecolon> Size \<rbrace> \<^bold>@\<^bold>G\<^bold>O\<^bold>A\<^bold>L G\<close>
+  \<open>\<^bold>p\<^bold>r\<^bold>o\<^bold>c op_const_size_t n \<lbrace> R \<longmapsto> R\<heavy_comma> SYNTHESIS \<^bold>v\<^bold>a\<^bold>l n \<Ztypecolon> Size \<rbrace> \<^bold>@\<^bold>G\<^bold>O\<^bold>A\<^bold>L G\<close>
   unfolding Synthesis_def GOAL_CTXT_def
   using op_const_size_t[THEN \<phi>frame, simplified] .
 
@@ -278,19 +279,20 @@ subsubsection \<open>Integer Arithmetic\<close>
 paragraph \<open>Addition\<close>
 
 lemma (in std) op_add[\<phi>overload +]:
-  \<open>\<^bold>p\<^bold>r\<^bold>e\<^bold>m\<^bold>i\<^bold>s\<^bold>e x + y < 2^b \<Longrightarrow> \<^bold>p\<^bold>r\<^bold>o\<^bold>c op_add b vy vx \<lbrace> x \<Ztypecolon> Val vx \<nat>[b]\<heavy_comma> y \<Ztypecolon> Val vy \<nat>[b] \<longmapsto> x + y \<Ztypecolon> \<^bold>v\<^bold>a\<^bold>l \<nat>[b] \<rbrace>\<close>
+  \<open> \<^bold>p\<^bold>r\<^bold>e\<^bold>m\<^bold>i\<^bold>s\<^bold>e x + y < 2^b
+\<Longrightarrow> \<^bold>p\<^bold>r\<^bold>o\<^bold>c op_add b (\<phi>V_pair vy vx) \<lbrace> x \<Ztypecolon> Val vx \<nat>[b]\<heavy_comma> y \<Ztypecolon> Val vy \<nat>[b] \<longmapsto> \<^bold>v\<^bold>a\<^bold>l x + y \<Ztypecolon> \<nat>[b] \<rbrace>\<close>
   unfolding op_add_def Premise_def
-  by \<phi>reason
+  by (cases vx; cases vy; simp, \<phi>reason)
 
-proc [
-    \<phi>reason on \<open>\<^bold>p\<^bold>r\<^bold>o\<^bold>c ?F \<lbrace> ?R \<longmapsto> ?R2\<heavy_comma> SYNTHESIS VAL (?x + ?y) \<Ztypecolon> ?T \<^bold>t\<^bold>h\<^bold>r\<^bold>o\<^bold>w\<^bold>s ?E \<rbrace> \<^bold>@\<^bold>G\<^bold>O\<^bold>A\<^bold>L ?G\<close>
+proc \<phi>__synthesis_add[
+    \<phi>reason on \<open>\<^bold>p\<^bold>r\<^bold>o\<^bold>c ?F \<lbrace> ?R \<longmapsto> ?R2\<heavy_comma> SYNTHESIS \<^bold>v\<^bold>a\<^bold>l (?x + ?y) \<Ztypecolon> ?T \<^bold>t\<^bold>h\<^bold>r\<^bold>o\<^bold>w\<^bold>s ?E \<rbrace> \<^bold>@\<^bold>G\<^bold>O\<^bold>A\<^bold>L ?G\<close>
 ]:
-  assumes F1: \<open>\<^bold>p\<^bold>r\<^bold>o\<^bold>c f1 \<lbrace> R \<longmapsto> R1\<heavy_comma> SYNTHESIS x \<Ztypecolon> \<nat>[b]  \<^bold>t\<^bold>h\<^bold>r\<^bold>o\<^bold>w\<^bold>s E1 \<rbrace>  \<^bold>@\<^bold>G\<^bold>O\<^bold>A\<^bold>L G\<close>
-    and   F2: \<open>\<^bold>p\<^bold>r\<^bold>o\<^bold>c f2 \<lbrace> R1 \<longmapsto> R2\<heavy_comma> SYNTHESIS y \<Ztypecolon> \<nat>[b] \<^bold>t\<^bold>h\<^bold>r\<^bold>o\<^bold>w\<^bold>s E2 \<rbrace>  \<^bold>@\<^bold>G\<^bold>O\<^bold>A\<^bold>L G\<close>
+  assumes F1: \<open>\<^bold>p\<^bold>r\<^bold>o\<^bold>c f1 \<lbrace> R \<longmapsto> R1\<heavy_comma> SYNTHESIS \<^bold>v\<^bold>a\<^bold>l x \<Ztypecolon> \<nat>[b]  \<^bold>t\<^bold>h\<^bold>r\<^bold>o\<^bold>w\<^bold>s E1 \<rbrace>  \<^bold>@\<^bold>G\<^bold>O\<^bold>A\<^bold>L G\<close>
+    and   F2: \<open>\<^bold>p\<^bold>r\<^bold>o\<^bold>c f2 \<lbrace> R1 \<longmapsto> R2\<heavy_comma> SYNTHESIS \<^bold>v\<^bold>a\<^bold>l y \<Ztypecolon> \<nat>[b] \<^bold>t\<^bold>h\<^bold>r\<^bold>o\<^bold>w\<^bold>s E2 \<rbrace>  \<^bold>@\<^bold>G\<^bold>O\<^bold>A\<^bold>L G\<close>
   premises \<open>x + y < 2 ^ b\<close>
   goal G
   argument \<open>R\<close>
-  return   \<open>R2\<heavy_comma> SYNTHESIS VAL (x + y) \<Ztypecolon> \<nat>[b]\<close>
+  return   \<open>R2\<heavy_comma> SYNTHESIS \<^bold>v\<^bold>a\<^bold>l (x + y) \<Ztypecolon> \<nat>[b]\<close>
   throws \<open>E1 + E2\<close>
   \<medium_left_bracket> F1 \<rightarrow> x;; F2 \<rightarrow> y;; $x $y + \<medium_right_bracket>. .
 
@@ -298,21 +300,22 @@ proc [
 paragraph \<open>Subtraction\<close>
 
 lemma (in std) op_sub[\<phi>overload -]:
-  \<open>\<^bold>p\<^bold>r\<^bold>e\<^bold>m\<^bold>i\<^bold>s\<^bold>e y \<le> x \<Longrightarrow> \<^bold>p\<^bold>r\<^bold>o\<^bold>c op_sub b vy vx \<lbrace> x \<Ztypecolon> Val vx \<nat>[b]\<heavy_comma> y \<Ztypecolon> Val vy \<nat>[b] \<longmapsto> x - y \<Ztypecolon> \<^bold>v\<^bold>a\<^bold>l \<nat>[b] \<rbrace>\<close>
+  \<open> \<^bold>p\<^bold>r\<^bold>e\<^bold>m\<^bold>i\<^bold>s\<^bold>e y \<le> x
+\<Longrightarrow> \<^bold>p\<^bold>r\<^bold>o\<^bold>c op_sub b (\<phi>V_pair vy vx) \<lbrace> x \<Ztypecolon> Val vx \<nat>[b]\<heavy_comma> y \<Ztypecolon> Val vy \<nat>[b] \<longmapsto> \<^bold>v\<^bold>a\<^bold>l x - y \<Ztypecolon> \<nat>[b] \<rbrace>\<close>
   unfolding op_sub_def Premise_def
-  apply \<phi>reason
+  apply (cases vx; cases vy; simp, \<phi>reason)
   apply (simp add: \<phi>expns)
   by (metis Nat.add_diff_assoc2 add.commute less_imp_diff_less mod_add_self2 mod_less)
 
-proc [
-    \<phi>reason on \<open>\<^bold>p\<^bold>r\<^bold>o\<^bold>c ?F \<lbrace> ?R \<longmapsto> ?R2\<heavy_comma> SYNTHESIS VAL (?x - ?y) \<Ztypecolon> ?T \<^bold>t\<^bold>h\<^bold>r\<^bold>o\<^bold>w\<^bold>s ?E \<rbrace> \<^bold>@\<^bold>G\<^bold>O\<^bold>A\<^bold>L ?G\<close>
+proc \<phi>__synthesis_sub[
+    \<phi>reason on \<open>\<^bold>p\<^bold>r\<^bold>o\<^bold>c ?F \<lbrace> ?R \<longmapsto> ?R2\<heavy_comma> SYNTHESIS \<^bold>v\<^bold>a\<^bold>l (?x - ?y) \<Ztypecolon> ?T \<^bold>t\<^bold>h\<^bold>r\<^bold>o\<^bold>w\<^bold>s ?E \<rbrace> \<^bold>@\<^bold>G\<^bold>O\<^bold>A\<^bold>L ?G\<close>
 ]:
-  assumes F1: \<open>\<^bold>p\<^bold>r\<^bold>o\<^bold>c f1 \<lbrace> R \<longmapsto> R1\<heavy_comma> SYNTHESIS x \<Ztypecolon> \<nat>[b] \<^bold>t\<^bold>h\<^bold>r\<^bold>o\<^bold>w\<^bold>s E1 \<rbrace>  \<^bold>@\<^bold>G\<^bold>O\<^bold>A\<^bold>L G\<close>
-    and   F2: \<open>\<^bold>p\<^bold>r\<^bold>o\<^bold>c f2 \<lbrace> R1 \<longmapsto> R2\<heavy_comma> SYNTHESIS y \<Ztypecolon> \<nat>[b] \<^bold>t\<^bold>h\<^bold>r\<^bold>o\<^bold>w\<^bold>s E2 \<rbrace>  \<^bold>@\<^bold>G\<^bold>O\<^bold>A\<^bold>L G\<close>
+  assumes F1: \<open>\<^bold>p\<^bold>r\<^bold>o\<^bold>c f1 \<lbrace> R \<longmapsto> R1\<heavy_comma> SYNTHESIS \<^bold>v\<^bold>a\<^bold>l x \<Ztypecolon> \<nat>[b] \<^bold>t\<^bold>h\<^bold>r\<^bold>o\<^bold>w\<^bold>s E1 \<rbrace>  \<^bold>@\<^bold>G\<^bold>O\<^bold>A\<^bold>L G\<close>
+    and   F2: \<open>\<^bold>p\<^bold>r\<^bold>o\<^bold>c f2 \<lbrace> R1 \<longmapsto> R2\<heavy_comma> SYNTHESIS \<^bold>v\<^bold>a\<^bold>l y \<Ztypecolon> \<nat>[b] \<^bold>t\<^bold>h\<^bold>r\<^bold>o\<^bold>w\<^bold>s E2 \<rbrace>  \<^bold>@\<^bold>G\<^bold>O\<^bold>A\<^bold>L G\<close>
   premises \<open>y \<le> x\<close>
   goal G
   argument \<open>R\<close>
-  return   \<open>R2\<heavy_comma> SYNTHESIS VAL (x - y) \<Ztypecolon> \<nat>[b]\<close>
+  return   \<open>R2\<heavy_comma> SYNTHESIS \<^bold>v\<^bold>a\<^bold>l (x - y) \<Ztypecolon> \<nat>[b]\<close>
   throws \<open>E1 + E2\<close>
   \<medium_left_bracket> F1 \<rightarrow> x;; F2 \<rightarrow> y;; $x $y - \<medium_right_bracket>. .
 
@@ -320,19 +323,19 @@ proc [
 paragraph \<open>Division\<close>
 
 lemma (in std) op_udiv[\<phi>overload /]:
-  \<open>\<^bold>p\<^bold>r\<^bold>o\<^bold>c op_udiv b vy vx \<lbrace> x \<Ztypecolon> Val vx \<nat>[b]\<heavy_comma> y \<Ztypecolon> Val vy \<nat>[b] \<longmapsto> x div y \<Ztypecolon> \<^bold>v\<^bold>a\<^bold>l \<nat>[b] \<rbrace>\<close>
+  \<open>\<^bold>p\<^bold>r\<^bold>o\<^bold>c op_udiv b (\<phi>V_pair vy vx) \<lbrace> x \<Ztypecolon> Val vx \<nat>[b]\<heavy_comma> y \<Ztypecolon> Val vy \<nat>[b] \<longmapsto> \<^bold>v\<^bold>a\<^bold>l x div y \<Ztypecolon> \<nat>[b] \<rbrace>\<close>
   unfolding op_udiv_def Premise_def
-  apply \<phi>reason apply (simp add: \<phi>expns)
+  apply (cases vx; cases vy; simp, \<phi>reason) apply (simp add: \<phi>expns)
   using div_le_dividend le_less_trans by blast
 
-proc [
-    \<phi>reason on \<open>\<^bold>p\<^bold>r\<^bold>o\<^bold>c ?F \<lbrace> ?R \<longmapsto> ?R2\<heavy_comma> SYNTHESIS VAL (?x div ?y) \<Ztypecolon> ?T \<^bold>t\<^bold>h\<^bold>r\<^bold>o\<^bold>w\<^bold>s ?E \<rbrace> \<^bold>@\<^bold>G\<^bold>O\<^bold>A\<^bold>L ?G\<close>
+proc \<phi>__synthesis_udiv[
+    \<phi>reason on \<open>\<^bold>p\<^bold>r\<^bold>o\<^bold>c ?F \<lbrace> ?R \<longmapsto> ?R2\<heavy_comma> SYNTHESIS \<^bold>v\<^bold>a\<^bold>l (?x div ?y) \<Ztypecolon> ?T \<^bold>t\<^bold>h\<^bold>r\<^bold>o\<^bold>w\<^bold>s ?E \<rbrace> \<^bold>@\<^bold>G\<^bold>O\<^bold>A\<^bold>L ?G\<close>
 ]:
-  assumes F1: \<open>\<^bold>p\<^bold>r\<^bold>o\<^bold>c f1 \<lbrace> R \<longmapsto> R1\<heavy_comma> SYNTHESIS x \<Ztypecolon> \<nat>[b] \<^bold>t\<^bold>h\<^bold>r\<^bold>o\<^bold>w\<^bold>s E1 \<rbrace>  \<^bold>@\<^bold>G\<^bold>O\<^bold>A\<^bold>L G\<close>
-    and   F2: \<open>\<^bold>p\<^bold>r\<^bold>o\<^bold>c f2 \<lbrace> R1 \<longmapsto> R2\<heavy_comma> SYNTHESIS y \<Ztypecolon> \<nat>[b] \<^bold>t\<^bold>h\<^bold>r\<^bold>o\<^bold>w\<^bold>s E2 \<rbrace>  \<^bold>@\<^bold>G\<^bold>O\<^bold>A\<^bold>L G\<close>
+  assumes F1: \<open>\<^bold>p\<^bold>r\<^bold>o\<^bold>c f1 \<lbrace> R \<longmapsto> R1\<heavy_comma> SYNTHESIS \<^bold>v\<^bold>a\<^bold>l x \<Ztypecolon> \<nat>[b] \<^bold>t\<^bold>h\<^bold>r\<^bold>o\<^bold>w\<^bold>s E1 \<rbrace>  \<^bold>@\<^bold>G\<^bold>O\<^bold>A\<^bold>L G\<close>
+    and   F2: \<open>\<^bold>p\<^bold>r\<^bold>o\<^bold>c f2 \<lbrace> R1 \<longmapsto> R2\<heavy_comma> SYNTHESIS \<^bold>v\<^bold>a\<^bold>l y \<Ztypecolon> \<nat>[b] \<^bold>t\<^bold>h\<^bold>r\<^bold>o\<^bold>w\<^bold>s E2 \<rbrace>  \<^bold>@\<^bold>G\<^bold>O\<^bold>A\<^bold>L G\<close>
   goal G
   argument \<open>R\<close>
-  return   \<open>R2\<heavy_comma> SYNTHESIS VAL (x div y) \<Ztypecolon> \<nat>[b]\<close>
+  return   \<open>R2\<heavy_comma> SYNTHESIS \<^bold>v\<^bold>a\<^bold>l (x div y) \<Ztypecolon> \<nat>[b]\<close>
   throws \<open>E1 + E2\<close>
   \<medium_left_bracket> F1 \<rightarrow> x;; F2 \<rightarrow> y;; $x $y / \<medium_right_bracket>. .
 
@@ -340,58 +343,58 @@ proc [
 paragraph \<open>Less Than\<close>
 
 lemma (in std) op_lt[\<phi>overload <]:
-  \<open>\<^bold>p\<^bold>r\<^bold>o\<^bold>c op_lt b \<lbrace> x \<Ztypecolon> \<nat>[b]\<heavy_comma> y \<Ztypecolon> \<nat>[b] \<longmapsto> x < y \<Ztypecolon> \<bool> \<rbrace>\<close>
+  \<open>\<^bold>p\<^bold>r\<^bold>o\<^bold>c op_lt b (\<phi>V_pair rawy rawx) \<lbrace> x \<Ztypecolon> Val rawx \<nat>[b]\<heavy_comma> y \<Ztypecolon> Val rawy \<nat>[b] \<longmapsto> \<^bold>v\<^bold>a\<^bold>l x < y \<Ztypecolon> \<bool> \<rbrace>\<close>
   unfolding op_lt_def
-  by \<phi>reason
+  by (cases rawx; cases rawy; simp, \<phi>reason)
 
-proc [
-    \<phi>reason on \<open>\<^bold>p\<^bold>r\<^bold>o\<^bold>c ?F \<lbrace> ?R \<longmapsto> ?R2\<heavy_comma> SYNTHESIS VAL (?x < ?y) \<Ztypecolon> ?T \<^bold>t\<^bold>h\<^bold>r\<^bold>o\<^bold>w\<^bold>s ?E \<rbrace> \<^bold>@\<^bold>G\<^bold>O\<^bold>A\<^bold>L ?G\<close>
+proc \<phi>__synthesis_lt[
+    \<phi>reason on \<open>\<^bold>p\<^bold>r\<^bold>o\<^bold>c ?F \<lbrace> ?R \<longmapsto> ?R2\<heavy_comma> SYNTHESIS \<^bold>v\<^bold>a\<^bold>l (?x < ?y) \<Ztypecolon> ?T \<^bold>t\<^bold>h\<^bold>r\<^bold>o\<^bold>w\<^bold>s ?E \<rbrace> \<^bold>@\<^bold>G\<^bold>O\<^bold>A\<^bold>L ?G\<close>
 ]:
-  assumes F1: \<open>\<^bold>p\<^bold>r\<^bold>o\<^bold>c f1 \<lbrace> R \<longmapsto> R1\<heavy_comma> SYNTHESIS x \<Ztypecolon> \<nat>[b] \<^bold>t\<^bold>h\<^bold>r\<^bold>o\<^bold>w\<^bold>s E1 \<rbrace>  \<^bold>@\<^bold>G\<^bold>O\<^bold>A\<^bold>L G\<close>
-    and   F2: \<open>\<^bold>p\<^bold>r\<^bold>o\<^bold>c f2 \<lbrace> R1 \<longmapsto> R2\<heavy_comma> SYNTHESIS y \<Ztypecolon> \<nat>[b] \<^bold>t\<^bold>h\<^bold>r\<^bold>o\<^bold>w\<^bold>s E2 \<rbrace>  \<^bold>@\<^bold>G\<^bold>O\<^bold>A\<^bold>L G\<close>
+  assumes F1: \<open>\<^bold>p\<^bold>r\<^bold>o\<^bold>c f1 \<lbrace> R \<longmapsto> R1\<heavy_comma> SYNTHESIS \<^bold>v\<^bold>a\<^bold>l x \<Ztypecolon> \<nat>[b] \<^bold>t\<^bold>h\<^bold>r\<^bold>o\<^bold>w\<^bold>s E1 \<rbrace>  \<^bold>@\<^bold>G\<^bold>O\<^bold>A\<^bold>L G\<close>
+    and   F2: \<open>\<^bold>p\<^bold>r\<^bold>o\<^bold>c f2 \<lbrace> R1 \<longmapsto> R2\<heavy_comma> SYNTHESIS \<^bold>v\<^bold>a\<^bold>l y \<Ztypecolon> \<nat>[b] \<^bold>t\<^bold>h\<^bold>r\<^bold>o\<^bold>w\<^bold>s E2 \<rbrace>  \<^bold>@\<^bold>G\<^bold>O\<^bold>A\<^bold>L G\<close>
   goal G
   argument \<open>R\<close>
-  return   \<open>R2\<heavy_comma> SYNTHESIS VAL (x < y) \<Ztypecolon> \<bool>\<close>
+  return   \<open>R2\<heavy_comma> SYNTHESIS \<^bold>v\<^bold>a\<^bold>l (x < y) \<Ztypecolon> \<bool>\<close>
   throws \<open>E1 + E2\<close>
   \<medium_left_bracket> F1 \<rightarrow> x;; F2 \<rightarrow> y ;; $x $y < \<medium_right_bracket>. .
 
-proc [
-    \<phi>reason on \<open>\<^bold>p\<^bold>r\<^bold>o\<^bold>c ?F \<lbrace> ?R \<longmapsto> ?R2\<heavy_comma> SYNTHESIS VAL (?x > ?y) \<Ztypecolon> ?T \<^bold>t\<^bold>h\<^bold>r\<^bold>o\<^bold>w\<^bold>s ?E \<rbrace> \<^bold>@\<^bold>G\<^bold>O\<^bold>A\<^bold>L ?G\<close>
+proc \<phi>__synthesis_gt[
+    \<phi>reason on \<open>\<^bold>p\<^bold>r\<^bold>o\<^bold>c ?F \<lbrace> ?R \<longmapsto> ?R2\<heavy_comma> SYNTHESIS \<^bold>v\<^bold>a\<^bold>l (?x > ?y) \<Ztypecolon> ?T \<^bold>t\<^bold>h\<^bold>r\<^bold>o\<^bold>w\<^bold>s ?E \<rbrace> \<^bold>@\<^bold>G\<^bold>O\<^bold>A\<^bold>L ?G\<close>
 ]:
-  assumes F1: \<open>\<^bold>p\<^bold>r\<^bold>o\<^bold>c f1 \<lbrace> R \<longmapsto> R1\<heavy_comma> SYNTHESIS x \<Ztypecolon> \<nat>[b] \<^bold>t\<^bold>h\<^bold>r\<^bold>o\<^bold>w\<^bold>s E1 \<rbrace>  \<^bold>@\<^bold>G\<^bold>O\<^bold>A\<^bold>L G\<close>
-    and   F2: \<open>\<^bold>p\<^bold>r\<^bold>o\<^bold>c f2 \<lbrace> R1 \<longmapsto> R2\<heavy_comma> SYNTHESIS y \<Ztypecolon> \<nat>[b] \<^bold>t\<^bold>h\<^bold>r\<^bold>o\<^bold>w\<^bold>s E2 \<rbrace>  \<^bold>@\<^bold>G\<^bold>O\<^bold>A\<^bold>L G\<close>
+  assumes F1: \<open>\<^bold>p\<^bold>r\<^bold>o\<^bold>c f1 \<lbrace> R \<longmapsto> R1\<heavy_comma> SYNTHESIS \<^bold>v\<^bold>a\<^bold>l x \<Ztypecolon> \<nat>[b] \<^bold>t\<^bold>h\<^bold>r\<^bold>o\<^bold>w\<^bold>s E1 \<rbrace>  \<^bold>@\<^bold>G\<^bold>O\<^bold>A\<^bold>L G\<close>
+    and   F2: \<open>\<^bold>p\<^bold>r\<^bold>o\<^bold>c f2 \<lbrace> R1 \<longmapsto> R2\<heavy_comma> SYNTHESIS \<^bold>v\<^bold>a\<^bold>l y \<Ztypecolon> \<nat>[b] \<^bold>t\<^bold>h\<^bold>r\<^bold>o\<^bold>w\<^bold>s E2 \<rbrace>  \<^bold>@\<^bold>G\<^bold>O\<^bold>A\<^bold>L G\<close>
   goal G
   argument \<open>R\<close>
-  return   \<open>R2\<heavy_comma> SYNTHESIS VAL (x > y) \<Ztypecolon> \<bool>\<close>
+  return   \<open>R2\<heavy_comma> SYNTHESIS \<^bold>v\<^bold>a\<^bold>l (x > y) \<Ztypecolon> \<bool>\<close>
   throws \<open>E1 + E2\<close>
   \<medium_left_bracket> F1 \<rightarrow> y;; F2 $y < \<medium_right_bracket>. .
 
 paragraph \<open>Less Equal\<close>
 
 lemma (in std) op_le[\<phi>overload \<le>]:
-  \<open>\<^bold>p\<^bold>r\<^bold>o\<^bold>c op_le b \<lbrace> x \<Ztypecolon> \<nat>[b]\<heavy_comma> y \<Ztypecolon> \<nat>[b] \<longmapsto> x \<le> y \<Ztypecolon> \<bool> \<rbrace>\<close>
+  \<open>\<^bold>p\<^bold>r\<^bold>o\<^bold>c op_le b (\<phi>V_pair rawy rawx) \<lbrace> x \<Ztypecolon> Val rawx \<nat>[b]\<heavy_comma> y \<Ztypecolon> Val rawy \<nat>[b] \<longmapsto> \<^bold>v\<^bold>a\<^bold>l x \<le> y \<Ztypecolon> \<bool> \<rbrace>\<close>
   unfolding op_le_def
-  by \<phi>reason
+  by (cases rawx; cases rawy; simp, \<phi>reason)
 
-proc [
-    \<phi>reason on \<open>\<^bold>p\<^bold>r\<^bold>o\<^bold>c ?F \<lbrace> ?R \<longmapsto> ?R2\<heavy_comma> SYNTHESIS VAL (?x \<le> ?y) \<Ztypecolon> ?T \<^bold>t\<^bold>h\<^bold>r\<^bold>o\<^bold>w\<^bold>s ?E \<rbrace> \<^bold>@\<^bold>G\<^bold>O\<^bold>A\<^bold>L ?G\<close>
+proc \<phi>__synthesis_le[
+    \<phi>reason on \<open>\<^bold>p\<^bold>r\<^bold>o\<^bold>c ?F \<lbrace> ?R \<longmapsto> ?R2\<heavy_comma> SYNTHESIS \<^bold>v\<^bold>a\<^bold>l (?x \<le> ?y) \<Ztypecolon> ?T \<^bold>t\<^bold>h\<^bold>r\<^bold>o\<^bold>w\<^bold>s ?E \<rbrace> \<^bold>@\<^bold>G\<^bold>O\<^bold>A\<^bold>L ?G\<close>
 ]:
-  assumes F1: \<open>\<^bold>p\<^bold>r\<^bold>o\<^bold>c f1 \<lbrace> R \<longmapsto> R1\<heavy_comma> SYNTHESIS x \<Ztypecolon> \<nat>[b]  \<^bold>t\<^bold>h\<^bold>r\<^bold>o\<^bold>w\<^bold>s E1 \<rbrace>  \<^bold>@\<^bold>G\<^bold>O\<^bold>A\<^bold>L G\<close>
-    and   F2: \<open>\<^bold>p\<^bold>r\<^bold>o\<^bold>c f2 \<lbrace> R1 \<longmapsto> R2\<heavy_comma> SYNTHESIS y \<Ztypecolon> \<nat>[b] \<^bold>t\<^bold>h\<^bold>r\<^bold>o\<^bold>w\<^bold>s E2 \<rbrace>  \<^bold>@\<^bold>G\<^bold>O\<^bold>A\<^bold>L G\<close>
+  assumes F1: \<open>\<^bold>p\<^bold>r\<^bold>o\<^bold>c f1 \<lbrace> R \<longmapsto> R1\<heavy_comma> SYNTHESIS \<^bold>v\<^bold>a\<^bold>l x \<Ztypecolon> \<nat>[b]  \<^bold>t\<^bold>h\<^bold>r\<^bold>o\<^bold>w\<^bold>s E1 \<rbrace>  \<^bold>@\<^bold>G\<^bold>O\<^bold>A\<^bold>L G\<close>
+    and   F2: \<open>\<^bold>p\<^bold>r\<^bold>o\<^bold>c f2 \<lbrace> R1 \<longmapsto> R2\<heavy_comma> SYNTHESIS \<^bold>v\<^bold>a\<^bold>l y \<Ztypecolon> \<nat>[b] \<^bold>t\<^bold>h\<^bold>r\<^bold>o\<^bold>w\<^bold>s E2 \<rbrace>  \<^bold>@\<^bold>G\<^bold>O\<^bold>A\<^bold>L G\<close>
   goal G
   argument \<open>R\<close>
-  return   \<open>R2\<heavy_comma> SYNTHESIS VAL (x \<le> y) \<Ztypecolon> \<bool>\<close>
+  return   \<open>R2\<heavy_comma> SYNTHESIS \<^bold>v\<^bold>a\<^bold>l (x \<le> y) \<Ztypecolon> \<bool>\<close>
   throws \<open>E1 + E2\<close>
   \<medium_left_bracket> F1 \<rightarrow> x;; F2 \<rightarrow> y;; $x $y \<le> \<medium_right_bracket>. .
 
-proc [
-    \<phi>reason on \<open>\<^bold>p\<^bold>r\<^bold>o\<^bold>c ?F \<lbrace> ?R \<longmapsto> ?R2\<heavy_comma> SYNTHESIS VAL (?x \<ge> ?y) \<Ztypecolon> ?T \<^bold>t\<^bold>h\<^bold>r\<^bold>o\<^bold>w\<^bold>s ?E \<rbrace> \<^bold>@\<^bold>G\<^bold>O\<^bold>A\<^bold>L ?G\<close>
+proc \<phi>__synthesis_ge[
+    \<phi>reason on \<open>\<^bold>p\<^bold>r\<^bold>o\<^bold>c ?F \<lbrace> ?R \<longmapsto> ?R2\<heavy_comma> SYNTHESIS \<^bold>v\<^bold>a\<^bold>l (?x \<ge> ?y) \<Ztypecolon> ?T \<^bold>t\<^bold>h\<^bold>r\<^bold>o\<^bold>w\<^bold>s ?E \<rbrace> \<^bold>@\<^bold>G\<^bold>O\<^bold>A\<^bold>L ?G\<close>
 ]:
-  assumes F1: \<open>\<^bold>p\<^bold>r\<^bold>o\<^bold>c f1 \<lbrace> R \<longmapsto> R1\<heavy_comma> SYNTHESIS x \<Ztypecolon> \<nat>[b] \<^bold>t\<^bold>h\<^bold>r\<^bold>o\<^bold>w\<^bold>s E1 \<rbrace>  \<^bold>@\<^bold>G\<^bold>O\<^bold>A\<^bold>L G\<close>
-    and   F2: \<open>\<^bold>p\<^bold>r\<^bold>o\<^bold>c f2 \<lbrace> R1 \<longmapsto> R2\<heavy_comma> SYNTHESIS y \<Ztypecolon> \<nat>[b] \<^bold>t\<^bold>h\<^bold>r\<^bold>o\<^bold>w\<^bold>s E2 \<rbrace>  \<^bold>@\<^bold>G\<^bold>O\<^bold>A\<^bold>L G\<close>
+  assumes F1: \<open>\<^bold>p\<^bold>r\<^bold>o\<^bold>c f1 \<lbrace> R \<longmapsto> R1\<heavy_comma> SYNTHESIS \<^bold>v\<^bold>a\<^bold>l x \<Ztypecolon> \<nat>[b] \<^bold>t\<^bold>h\<^bold>r\<^bold>o\<^bold>w\<^bold>s E1 \<rbrace>  \<^bold>@\<^bold>G\<^bold>O\<^bold>A\<^bold>L G\<close>
+    and   F2: \<open>\<^bold>p\<^bold>r\<^bold>o\<^bold>c f2 \<lbrace> R1 \<longmapsto> R2\<heavy_comma> SYNTHESIS \<^bold>v\<^bold>a\<^bold>l y \<Ztypecolon> \<nat>[b] \<^bold>t\<^bold>h\<^bold>r\<^bold>o\<^bold>w\<^bold>s E2 \<rbrace>  \<^bold>@\<^bold>G\<^bold>O\<^bold>A\<^bold>L G\<close>
   goal G
   argument \<open>R\<close>
-  return   \<open>R2\<heavy_comma> SYNTHESIS VAL (x \<ge> y) \<Ztypecolon> \<bool>\<close>
+  return   \<open>R2\<heavy_comma> SYNTHESIS \<^bold>v\<^bold>a\<^bold>l (x \<ge> y) \<Ztypecolon> \<bool>\<close>
   throws \<open>E1 + E2\<close>
   \<medium_left_bracket> F1 \<rightarrow> x;; F2 $x \<le> \<medium_right_bracket>. .
 
@@ -405,28 +408,29 @@ lemma (in std) op_equal_\<phi>app[\<phi>overload =]:
 \<Longrightarrow> \<phi>SemType (b \<Ztypecolon> T) TY
 \<Longrightarrow> \<phi>Equal T can_eq eq
 \<Longrightarrow> \<^bold>p\<^bold>r\<^bold>e\<^bold>m\<^bold>i\<^bold>s\<^bold>e can_eq a b
-\<Longrightarrow> \<^bold>p\<^bold>r\<^bold>o\<^bold>c op_equal TY \<lbrace> a \<Ztypecolon> T\<heavy_comma> b \<Ztypecolon> T \<longmapsto> eq a b \<Ztypecolon> \<bool> \<rbrace>\<close>
+\<Longrightarrow> \<^bold>p\<^bold>r\<^bold>o\<^bold>c op_equal TY (\<phi>V_pair rawb rawa) \<lbrace> a \<Ztypecolon> Val rawa T\<heavy_comma> b \<Ztypecolon> Val rawb T \<longmapsto> \<^bold>v\<^bold>a\<^bold>l eq a b \<Ztypecolon> \<bool> \<rbrace>\<close>
   unfolding op_equal_def
-  apply \<phi>reason
-    apply (simp add: \<phi>SemType_def subset_iff)
-   apply \<phi>reason
-    apply (simp add: \<phi>SemType_def subset_iff)
-apply (unfold \<phi>Equal_def Premise_def, simp)
-  by \<phi>reason
+  apply (cases rawa; cases rawb; simp, \<phi>reason)
+    apply (simp add: \<phi>SemType_def subset_iff Premise_def, \<phi>reason)
+    apply (simp add: \<phi>SemType_def subset_iff Premise_def, \<phi>reason)
+   apply (unfold \<phi>Equal_def Premise_def, simp)
+  apply (rule \<phi>M_Success')
+  by (\<phi>reason)
 
 
-proc [
-    \<phi>reason on \<open>\<^bold>p\<^bold>r\<^bold>o\<^bold>c ?F \<lbrace> ?R \<longmapsto> ?R2\<heavy_comma> SYNTHESIS VAL (?x = ?y) \<Ztypecolon> ?T \<^bold>t\<^bold>h\<^bold>r\<^bold>o\<^bold>w\<^bold>s ?E \<rbrace> \<^bold>@\<^bold>G\<^bold>O\<^bold>A\<^bold>L ?G\<close>
+
+proc \<phi>__synthesis_eq[
+    \<phi>reason on \<open>\<^bold>p\<^bold>r\<^bold>o\<^bold>c ?F \<lbrace> ?R \<longmapsto> ?R2\<heavy_comma> SYNTHESIS \<^bold>v\<^bold>a\<^bold>l (?x = ?y) \<Ztypecolon> ?T \<^bold>t\<^bold>h\<^bold>r\<^bold>o\<^bold>w\<^bold>s ?E \<rbrace> \<^bold>@\<^bold>G\<^bold>O\<^bold>A\<^bold>L ?G\<close>
 ]:
-  assumes F1: \<open>\<^bold>p\<^bold>r\<^bold>o\<^bold>c f1 \<lbrace> R \<longmapsto> R1\<heavy_comma> SYNTHESIS VAL x \<Ztypecolon> T  \<^bold>t\<^bold>h\<^bold>r\<^bold>o\<^bold>w\<^bold>s E1 \<rbrace>  \<^bold>@\<^bold>G\<^bold>O\<^bold>A\<^bold>L G\<close>
-    and   F2: \<open>\<^bold>p\<^bold>r\<^bold>o\<^bold>c f2 \<lbrace> R1 \<longmapsto> R2\<heavy_comma> SYNTHESIS VAL y \<Ztypecolon> T \<^bold>t\<^bold>h\<^bold>r\<^bold>o\<^bold>w\<^bold>s E2 \<rbrace>  \<^bold>@\<^bold>G\<^bold>O\<^bold>A\<^bold>L G\<close>
+  assumes F1: \<open>\<^bold>p\<^bold>r\<^bold>o\<^bold>c f1 \<lbrace> R  \<longmapsto> R1\<heavy_comma> SYNTHESIS \<^bold>v\<^bold>a\<^bold>l x \<Ztypecolon> T  \<^bold>t\<^bold>h\<^bold>r\<^bold>o\<^bold>w\<^bold>s E1 \<rbrace>  \<^bold>@\<^bold>G\<^bold>O\<^bold>A\<^bold>L G\<close>
+    and   F2: \<open>\<^bold>p\<^bold>r\<^bold>o\<^bold>c f2 \<lbrace> R1 \<longmapsto> R2\<heavy_comma> SYNTHESIS \<^bold>v\<^bold>a\<^bold>l y \<Ztypecolon> T \<^bold>t\<^bold>h\<^bold>r\<^bold>o\<^bold>w\<^bold>s E2 \<rbrace>  \<^bold>@\<^bold>G\<^bold>O\<^bold>A\<^bold>L G\<close>
   assumes [\<phi>reason on \<open>\<phi>SemType (x \<Ztypecolon> T) ?TY\<close>]: \<open>\<phi>SemType (x \<Ztypecolon> T) TY\<close>
     and   [\<phi>reason on \<open>\<phi>SemType (y \<Ztypecolon> T) ?TY\<close>]: \<open>\<phi>SemType (y \<Ztypecolon> T) TY\<close>
     and   [\<phi>reason on \<open>\<phi>Equal T ?can_eq ?eq\<close>]: \<open>\<phi>Equal T can_eq (=)\<close>
   premises \<open>can_eq x y\<close>
   goal G
   argument \<open>R\<close>
-  return   \<open>R2\<heavy_comma> SYNTHESIS VAL (x = y) \<Ztypecolon> \<bool>\<close>
+  return   \<open>R2\<heavy_comma> SYNTHESIS \<^bold>v\<^bold>a\<^bold>l (x = y) \<Ztypecolon> \<bool>\<close>
   throws \<open>E1 + E2\<close>
   \<medium_left_bracket> F1 \<rightarrow> x;; F2 \<rightarrow> y;; $x $y = \<medium_right_bracket>. .
 
@@ -439,29 +443,37 @@ subsection \<open>Branches & Loops\<close>
 
 context std begin
 
+
 lemma op_sel_\<phi>app:
-  \<open>\<^bold>p\<^bold>r\<^bold>o\<^bold>c op_sel \<lbrace> VAL A\<heavy_comma> VAL B\<heavy_comma> c \<Ztypecolon> \<bool> \<longmapsto> VAL (if c then A else B) \<rbrace>\<close>
+  \<open> \<phi>SemType (a \<Ztypecolon> A) TY
+\<Longrightarrow> \<phi>SemType (b \<Ztypecolon> B) TY
+\<Longrightarrow> \<^bold>p\<^bold>r\<^bold>o\<^bold>c op_sel TY (\<phi>V_pair rawc (\<phi>V_pair rawb rawa))
+      \<lbrace> a \<Ztypecolon> Val rawa A\<heavy_comma> b \<Ztypecolon> Val rawb B\<heavy_comma> c \<Ztypecolon> Val rawc \<bool> \<longmapsto> \<^bold>v\<^bold>a\<^bold>l (if c then a else b) \<Ztypecolon> (if c then A else B) \<rbrace>\<close>
   unfolding op_sel_def
-  by \<phi>reason
+  by (cases rawc; cases rawb; cases rawa; cases c; simp add: \<phi>SemType_def subset_iff, \<phi>reason)
 
 lemma branch_\<phi>app:
-  \<open> (\<^bold>p\<^bold>r\<^bold>e\<^bold>m\<^bold>i\<^bold>s\<^bold>e C \<longrightarrow> \<^bold>p\<^bold>r\<^bold>o\<^bold>c br\<^sub>T \<lbrace> X \<longmapsto> Y\<^sub>T \<^bold>t\<^bold>h\<^bold>r\<^bold>o\<^bold>w\<^bold>s E\<^sub>T \<rbrace>)
+  \<open> (\<^bold>p\<^bold>r\<^bold>e\<^bold>m\<^bold>i\<^bold>s\<^bold>e   C \<longrightarrow> \<^bold>p\<^bold>r\<^bold>o\<^bold>c br\<^sub>T \<lbrace> X \<longmapsto> Y\<^sub>T \<^bold>t\<^bold>h\<^bold>r\<^bold>o\<^bold>w\<^bold>s E\<^sub>T \<rbrace>)
 \<Longrightarrow> (\<^bold>p\<^bold>r\<^bold>e\<^bold>m\<^bold>i\<^bold>s\<^bold>e \<not> C \<longrightarrow> \<^bold>p\<^bold>r\<^bold>o\<^bold>c br\<^sub>F \<lbrace> X \<longmapsto> Y\<^sub>F \<^bold>t\<^bold>h\<^bold>r\<^bold>o\<^bold>w\<^bold>s E\<^sub>F \<rbrace>)
-\<Longrightarrow> \<^bold>c\<^bold>o\<^bold>n\<^bold>v Merge C Y\<^sub>T Y\<^sub>F = Y
-\<Longrightarrow> \<^bold>p\<^bold>r\<^bold>o\<^bold>c op_if br\<^sub>T br\<^sub>F \<lbrace> X\<heavy_comma> C \<Ztypecolon> \<bool> \<longmapsto> Y \<^bold>t\<^bold>h\<^bold>r\<^bold>o\<^bold>w\<^bold>s E\<^sub>T + E\<^sub>F \<rbrace>\<close>
+\<Longrightarrow> \<^bold>c\<^bold>o\<^bold>n\<^bold>v[branch_convergence] Merge C Y\<^sub>T Y\<^sub>F = Y
+\<Longrightarrow> \<^bold>p\<^bold>r\<^bold>o\<^bold>c op_if br\<^sub>T br\<^sub>F rawc \<lbrace> X\<heavy_comma> C \<Ztypecolon> Val rawc \<bool> \<longmapsto> Y \<^bold>t\<^bold>h\<^bold>r\<^bold>o\<^bold>w\<^bold>s E\<^sub>T + E\<^sub>F \<rbrace>\<close>
   unfolding op_if_def Premise_def Conv_def Merge_def
-  apply \<phi>reason apply (simp add: \<phi>expns)+
-  by (meson \<phi>CONSEQ plus_set_in_iff subsetI)
+  apply (cases rawc; cases C; simp; \<phi>reason; simp add: \<phi>expns)
+  using \<phi>CONSEQ'E cast_id subty_union by blast+
+
 
 proc "if":
-  assumes C: \<open>\<^bold>p\<^bold>r\<^bold>o\<^bold>c cond \<lbrace> X \<longmapsto> X1\<heavy_comma> C \<Ztypecolon> \<bool> \<^bold>t\<^bold>h\<^bold>r\<^bold>o\<^bold>w\<^bold>s E \<rbrace>\<close>
-      and brT: \<open>\<^bold>p\<^bold>r\<^bold>e\<^bold>m\<^bold>i\<^bold>s\<^bold>e C \<longrightarrow> \<^bold>p\<^bold>r\<^bold>o\<^bold>c brT \<lbrace> X1 \<longmapsto> Y\<^sub>T \<^bold>t\<^bold>h\<^bold>r\<^bold>o\<^bold>w\<^bold>s E\<^sub>T \<rbrace>\<close>
-      and brF: \<open>\<^bold>p\<^bold>r\<^bold>e\<^bold>m\<^bold>i\<^bold>s\<^bold>e \<not> C \<longrightarrow> \<^bold>p\<^bold>r\<^bold>o\<^bold>c brF \<lbrace> X1 \<longmapsto> Y\<^sub>F \<^bold>t\<^bold>h\<^bold>r\<^bold>o\<^bold>w\<^bold>s E\<^sub>F \<rbrace>\<close>
-      and [\<phi>reason on \<open>\<^bold>c\<^bold>o\<^bold>n\<^bold>v Merge C Y\<^sub>T Y\<^sub>F = ?Y\<close>]: \<open>\<^bold>c\<^bold>o\<^bold>n\<^bold>v Merge C Y\<^sub>T Y\<^sub>F = Y\<close>
+  assumes C: \<open>\<^bold>p\<^bold>r\<^bold>o\<^bold>c cond \<lbrace> X \<longmapsto> X1 (ret::'a sem_value)\<heavy_comma> \<^bold>v\<^bold>a\<^bold>l C \<Ztypecolon> \<bool> \<^bold>t\<^bold>h\<^bold>r\<^bold>o\<^bold>w\<^bold>s E \<rbrace>\<close>
+      and brT: \<open>\<forall>arg. \<^bold>p\<^bold>r\<^bold>e\<^bold>m\<^bold>i\<^bold>s\<^bold>e   C \<longrightarrow> \<^bold>p\<^bold>r\<^bold>o\<^bold>c brT \<lbrace> X1 arg \<longmapsto> Y\<^sub>T (ret::'a sem_value) \<^bold>t\<^bold>h\<^bold>r\<^bold>o\<^bold>w\<^bold>s E\<^sub>T \<rbrace>\<close>
+      and brF: \<open>\<forall>arg. \<^bold>p\<^bold>r\<^bold>e\<^bold>m\<^bold>i\<^bold>s\<^bold>e \<not> C \<longrightarrow> \<^bold>p\<^bold>r\<^bold>o\<^bold>c brF \<lbrace> X1 arg \<longmapsto> Y\<^sub>F (ret::'a sem_value) \<^bold>t\<^bold>h\<^bold>r\<^bold>o\<^bold>w\<^bold>s E\<^sub>F \<rbrace>\<close>
+      and [\<phi>reason on \<open>\<^bold>c\<^bold>o\<^bold>n\<^bold>v[branch_convergence] Merge C Y\<^sub>T Y\<^sub>F = ?Y\<close>]:
+              \<open>\<^bold>c\<^bold>o\<^bold>n\<^bold>v[branch_convergence] Merge C Y\<^sub>T Y\<^sub>F = Y\<close>
   argument \<open>X\<close>
-  return \<open>Y\<close>
+  return \<open>Y (ret::'a sem_value)\<close>
   throws \<open>E + E\<^sub>T + E\<^sub>F\<close>
-  \<medium_left_bracket> C branch brT brF \<medium_right_bracket>. .
+  \<medium_left_bracket> ;; C;; branch
+  note [ [\<phi>trace_reasoning] ]
+  ;; brT;; brF \<medium_right_bracket> .. .
 
 end
 
@@ -512,7 +524,6 @@ lemma (in std)
 
 declare [[\<phi>not_define_new_const]]
 
-declare [ [\<phi>trace_reasoning] ]
 
 proc (in std) do_while:
 assumes V: \<open>Variant_Cast vars X X'\<close>
